term.v
@@ -7,19 +7,12 @@ Require Import Coq.Setoids.Setoid.
 Require Import Coq.Classes.SetoidClass.
 Require Import FunInd.
 Require Import Recdef.
-Require Coq.Structures.OrdersAlt.
-Require Coq.Structures.OrderedTypeEx.
-Require Coq.MSets.MSetAVL.
-Require Coq.MSets.MSetInterface.
-Require Coq.FSets.FMapList.
 
 Import IfNotations.
 Import ListNotations.
 Open Scope string_scope.
 
 Close Scope nat.
-
-Module F := FMapList.Make OrderedTypeEx.String_as_OT.
 
 Reserved Notation "⟨ x , y , .. , z ⟩".
 
@@ -113,941 +106,60 @@ Proof.
   decide equality.
 Defined.
 
-Definition ctx := list (string * tm).
-
-Inductive maps: ctx → string → tm → Prop :=
-| maps_head {Γ x τ}: maps ((x, τ) :: Γ) x τ
-| maps_tail {Γ x y τ τ0}:
-    y ≠ x →
-    maps Γ x τ →
-    maps ((y, τ0) :: Γ) x τ
-.
-
-Fixpoint lookup (Γ: ctx) (x:string) :=
-  match Γ with
-  | (y, τ) :: Γ' =>
-    if string_dec y x then Some τ else lookup Γ' x
-  | _ => None
-  end.
-
-Theorem lookup_complete {Γ x τ}:
-  maps Γ x τ →
-  lookup Γ x = Some τ.
-Proof.
-  intro p.
-  induction p.
-  - cbn in *.
-    destruct (string_dec x x).
-    2: contradiction.
-    reflexivity.
-  - cbn in *.
-    destruct (string_dec y x).
-    + subst.
-      contradiction.
-    + assumption.
-Qed.
-
-Theorem lookup_sound {Γ x τ}:
-  lookup Γ x = Some τ →
-  maps Γ x τ.
-Proof.
-  intro p.
-  induction Γ.
-  1: discriminate.
-  destruct a as [y τ'].
-  cbn in p.
-  destruct (string_dec y x).
-  - subst.
-    inversion p.
-    subst.
-    constructor.
-  - constructor.
-    + assumption.
-    + apply IHΓ.
-      assumption.
-Defined.
-
-Reserved Notation "Γ ⊢ e ∈ τ" (at level 80).
-
-Inductive judge (Γ: ctx): tm → tm → Type :=
-| judge_var x τ:
-    maps Γ x τ →
-    Γ ⊢ var x ∈ τ
-
-| judge_set:
-    Γ ⊢ set ∈ type
-| judge_unit:
-    Γ ⊢ unit ∈ set
-| judge_prod A B:
-    Γ ⊢ A ∈ set → Γ ⊢ B ∈ set →
-    Γ ⊢ prod A B ∈ set
-| judge_exp A B:
-    Γ ⊢ A ∈ set → Γ ⊢ B ∈ set →
-    Γ ⊢ exp A B ∈ set
-| judge_pos κ A:
-    Γ ⊢ A ∈ set →
-    Γ ⊢ ◇ κ, A ∈ set
-| judge_nec κ A:
-    Γ ⊢ A ∈ set →
-    Γ ⊢ □ κ, A ∈ set
-| judge_eq κ0 κ1:
-    Γ ⊢ (κ0 ~ κ1) ∈ set
-
-| judge_tt:
-    Γ ⊢ tt ∈ unit
-| judge_fanout e0 e1 τ0 τ1:
-    Γ ⊢ e0 ∈ τ0 → Γ ⊢ e1 ∈ τ1 →
-    Γ ⊢ fanout e0 e1 ∈ (τ0 × τ1)
-
-| judge_π1 e τ0 τ1:
-    Γ ⊢ e ∈ (τ0 × τ1) →
-    Γ ⊢ π1 e ∈ τ0
-| judge_π2 e τ0 τ1:
-    Γ ⊢ e ∈ (τ0 × τ1) →
-    Γ ⊢ π2 e ∈ τ1
-
-| judge_lam e τ0 τ1 x:
-    (x, τ0) :: Γ ⊢ e ∈ τ1 →
-    Γ ⊢ lam x τ0 e ∈ [τ0, τ1]
-| judge_app e0 e1 τ0 τ1:
-    Γ ⊢ e0 ∈ [τ0, τ1] → Γ ⊢ e1 ∈ τ0 →
-    Γ ⊢ app e0 e1 ∈ τ1
-
-| judge_necessity κ e τ:
-    [] ⊢ e ∈ τ →
-    Γ ⊢ necessity κ e ∈ (□ κ, τ)
-
-| judge_ext κ e τ:
-    Γ ⊢ e ∈ (□ κ, τ) →
-    Γ ⊢ ext κ e ∈ τ
-| judge_dup κ e τ:
-    Γ ⊢ e ∈ (□ κ, τ) →
-    Γ ⊢ dup e ∈ (□ κ, □ κ, τ)
-
-| judge_box κ e τ:
-    Γ ⊢ e ∈ τ →
-    Γ ⊢ box κ e ∈ (◇ κ, τ)
-
-| judge_bind e0 e1 x κ τ0 τ1:
-    Γ ⊢ e0 ∈ (◇ κ, τ0) → (x, τ0) :: Γ ⊢ e1 ∈ (◇ κ, τ1) →
-    Γ ⊢ bind e0 x e1 ∈ (◇ κ, τ1)
-
-| judge_id κ:
-    Γ ⊢ id κ ∈ (κ ~ κ)
-
-| judge_compose e0 e1 κ0 κ1 κ2:
-    Γ ⊢ e0 ∈ (κ1 ~ κ2) → Γ ⊢ e1 ∈ (κ0 ~ κ1) →
-    Γ ⊢ (e0 ∘ e1) ∈ (κ0 ~ κ2)
-
-| judge_sym e κ0 κ1:
-    Γ ⊢ e ∈ (κ1 ~ κ0) →
-    Γ ⊢ sym e ∈ (κ0 ~ κ1)
-
-(* Really unsure of these as faithful to cylindrical logic *)
-| judge_cast_pos e0 e1 κ0 κ1 τ:
-      Γ ⊢ e0 ∈ (κ0 ~ κ1) → Γ ⊢ e1 ∈ (◇ κ0, τ) →
-      Γ ⊢ cast_pos e0 e1 ∈ (◇ κ1, τ)
-| judge_cast_nec e0 e1 κ0 κ1 τ:
-    Γ ⊢ e0 ∈ (κ0 ~ κ1) →
-    Γ ⊢ e1 ∈ (□ κ0, τ) →
-    Γ ⊢ cast_nec e0 e1 ∈ (□ κ1, τ)
-where "Γ ⊢ e ∈ τ" := (judge Γ e τ).
-
-Record ofty (τ: tm) := {
-  term: tm ;
-  proof: [] ⊢ term ∈ τ ;
-}.
-
-Arguments term {τ}.
-Arguments proof {τ}.
-Coercion term: ofty >-> tm.
-
-Fixpoint infer (Γ: ctx) (e: tm): option tm :=
-  match e with
-  | type => None
-
-  | set => Some type
-
-  | unit => Some set
-  | prod A B =>
-    infer Γ A >>= λ A',
-    infer Γ B >>= λ B',
-    (if A' is set then Some tt else None) >>
-    (if B' is set then Some tt else None) >>
-    Some set
-
-  | exp A B =>
-    infer Γ A >>= λ A',
-    infer Γ B >>= λ B',
-    (if A' is set then Some tt else None) >>
-    (if B' is set then Some tt else None) >>
-    Some set
-
-  | (◇ _, A) =>
-    infer Γ A >>= λ A',
-    (if A' is set then Some tt else None) >>
-    Some set
-  | (□ _, A) =>
-    infer Γ A >>= λ A',
-    (if A' is set then Some tt else None) >>
-    Some set
-
-  | (_ ~ _) => Some set
-
-  | var x => lookup Γ x
-
-  | lam x τ0 e =>
-    infer ((x, τ0) :: Γ) e >>= λ τ1,
-    Some [τ0, τ1]
-
-  | app e0 e1 =>
-    infer Γ e0 >>= λ A,
-    infer Γ e1 >>= λ τ0',
-    (if A is [τ0, τ1] then Some (τ0, τ1) else None) >>= λ '(τ0, τ1),
-    (if tm_eq τ0 τ0' then Some tt else None) >>
-    Some τ1
-
-  | tt => Some unit
-
-  | fanout e0 e1 =>
-    infer Γ e0 >>= λ τ0,
-    infer Γ e1 >>= λ τ1,
-    Some (τ0 × τ1)
-
-  | π1 e =>
-    infer Γ e >>= λ A,
-    if A is (τ0 × τ1)
-    then Some τ0
-    else None
-
-  | π2 e =>
-    infer Γ e >>= λ A,
-    if A is (τ0 × τ1)
-    then Some τ1
-    else None
-
-  | necessity κ e =>
-    infer [] e >>= λ τ,
-    Some (□ κ, τ)
-
-  | ext κ e =>
-    infer Γ e >>= λ A,
-    (if A is (□ κ', τ) then Some (κ', τ) else None) >>= λ '(κ', τ),
-    (if string_dec κ κ' then Some tt else None) >>
-    Some τ
-  | dup e =>
-    infer Γ e >>= λ A,
-    (if A is (□ κ, τ) then Some (κ, τ) else None) >>= λ '(κ, τ),
-    Some (□ κ, □ κ, τ)
-
-  | box κ e =>
-    infer Γ e >>= λ τ,
-    Some (◇ κ, τ)
-
-  | bind e0 x e1 =>
-    infer Γ e0 >>= λ A,
-    (if A is (◇ κ0, τ0) then Some (κ0, τ0) else None) >>= λ '(κ0, τ0),
-    infer ((x, τ0) :: Γ) e1 >>= λ B,
-    (if B is (◇ κ1, τ1) then Some (κ1, τ1) else None) >>= λ '(κ1, τ1),
-    (if string_dec κ0 κ1 then Some tt else None) >>
-    Some (◇ κ1, τ1)
-
-  | id κ => Some (κ ~ κ)
-  | e0 ∘ e1 =>
-    infer Γ e0 >>= λ A,
-    infer Γ e1 >>= λ B,
-    (if A is κ1 ~ κ2 then Some (κ1, κ2) else None) >>= λ '(κ1, κ2),
-    (if B is κ0 ~ κ1' then Some (κ0, κ1') else None) >>= λ '(κ0, κ1'),
-    (if string_dec κ1 κ1' then Some tt else None) >>
-    Some (κ0 ~ κ2)
-
-  | sym e =>
-    infer Γ e >>= λ A,
-    (if A is κ0 ~ κ1 then Some (κ0, κ1) else None) >>= λ '(κ0, κ1),
-    Some (κ1 ~ κ0)
-
-  | cast_pos e0 e1 =>
-    infer Γ e0 >>= λ A,
-    infer Γ e1 >>= λ B,
-    (if A is κ0 ~ κ1 then Some (κ0, κ1) else None) >>= λ '(κ0, κ1),
-    (if B is ◇ κ0', τ then Some (κ0', τ) else None) >>= λ '(κ0', τ),
-    (if string_dec κ0 κ0' then Some tt else None) >>
-    Some (◇ κ1, τ)
-
-  | cast_nec e0 e1 =>
-    infer Γ e0 >>= λ A,
-    infer Γ e1 >>= λ B,
-    (if A is κ0 ~ κ1 then Some (κ0, κ1) else None) >>= λ '(κ0, κ1),
-    (if B is □ κ0', τ then Some (κ0', τ) else None) >>= λ '(κ0', τ),
-    (if string_dec κ0 κ0' then Some tt else None) >>
-    Some (□ κ1, τ)
-  end.
-
-Theorem infer_complete {Γ e τ}:
-  Γ ⊢ e ∈ τ → infer Γ e = Some τ.
-  intro p.
-  induction p.
-  all: cbn in *.
-  all: auto.
-  all: try rewrite IHp.
-  all: cbn in *.
-  all: try rewrite IHp1.
-  all: cbn in *.
-  all: try rewrite IHp2.
-  all: cbn in *.
-  all: try reflexivity.
-  all: cbn in *.
-  - apply lookup_complete.
-    assumption.
-  - destruct (tm_eq τ0 τ0).
-    2: contradiction.
-    reflexivity.
-  - destruct (string_dec κ κ).
-    2: contradiction.
-    reflexivity.
-  - destruct (string_dec κ κ).
-    2: contradiction.
-    reflexivity.
-  - destruct (string_dec κ1 κ1).
-    2: contradiction.
-    reflexivity.
-  - destruct (string_dec κ0 κ0).
-    2: contradiction.
-    reflexivity.
-  - destruct (string_dec κ0 κ0).
-    2: contradiction.
-    reflexivity.
-Qed.
-
-Theorem infer_sound {Γ e τ}:
-  infer Γ e = Some τ → Γ ⊢ e ∈ τ.
-Proof.
-  generalize dependent Γ.
-  generalize dependent τ.
-  induction e.
-  all: intros τ Γ p.
-  all: cbn in *.
-  all: try discriminate.
-  - apply judge_var.
-    apply lookup_sound.
-    assumption.
-  - inversion p.
-    subst.
-    constructor.
-  - inversion p.
-    subst.
-    constructor.
-  - destruct (infer Γ e1) as [A|] eqn:A', (infer Γ e2) as [B|] eqn:B'.
-    all: try discriminate.
-    destruct A, B.
-    all: try discriminate.
-    cbn in p.
-    inversion p.
-    subst.
-    constructor.
-    + apply IHe1.
-      assumption.
-    + apply IHe2.
-      assumption.
-  - destruct (infer Γ e1) as [A|] eqn:A', (infer Γ e2) as [B|] eqn:B'.
-    all: try discriminate.
-    destruct A, B.
-    all: try discriminate.
-    cbn in p.
-    inversion p.
-    subst.
-    constructor.
-    + apply IHe1.
-      assumption.
-    + apply IHe2.
-      assumption.
-  - destruct (infer Γ e) as [A|] eqn:A'.
-    all: try discriminate.
-    destruct A.
-    all: try discriminate.
-    cbn in p.
-    inversion p.
-    subst.
-    constructor.
-    apply IHe.
-    assumption.
-  - destruct (infer Γ e) as [A|] eqn:A'.
-    all: try discriminate.
-    destruct A.
-    all: try discriminate.
-    cbn in p.
-    inversion p.
-    subst.
-    constructor.
-    apply IHe.
-    assumption.
-  - inversion p.
-    subst.
-    constructor.
-  - destruct (infer ((x, e1) :: Γ) e2) eqn:q.
-    2: discriminate.
-    inversion p.
-    subst.
-    apply judge_lam.
-    apply IHe2.
-    apply q.
-  - destruct (infer Γ e1) eqn:q1.
-    all: try discriminate.
-    cbn in *.
-    destruct (infer Γ e2) eqn:q2.
-    all: try discriminate.
-    cbn in *.
-    destruct t.
-    all: try discriminate.
-    cbn in *.
-    destruct (tm_eq t1 t0).
-    all: try discriminate.
-    cbn in *.
-    inversion p.
-    subst.
-    eapply judge_app.
-    Unshelve.
-    3: apply t0.
-    + apply IHe1.
-      apply q1.
-    + apply IHe2.
-      apply q2.
-  - inversion p.
-    subst.
-    apply judge_tt.
-  - destruct (infer Γ e1) eqn:q1.
-    all: try discriminate.
-    destruct (infer Γ e2) eqn:q2.
-    all: try discriminate.
-    inversion p.
-    subst.
-    apply judge_fanout.
-    + apply IHe1.
-      assumption.
-    + apply IHe2.
-      assumption.
-  - destruct (infer Γ e) eqn:q.
-    all: try discriminate.
-    destruct t.
-    all: try discriminate.
-    eapply judge_π1.
-    Unshelve.
-    2: apply t2.
-    inversion p.
-    subst.
-    apply IHe.
-    assumption.
-  - destruct (infer Γ e) eqn:q.
-    all: try discriminate.
-    destruct t.
-    all: try discriminate.
-    eapply judge_π2.
-    Unshelve.
-    2: apply t1.
-    inversion p.
-    subst.
-    apply IHe.
-    assumption.
-  - destruct (infer [] e) eqn:q.
-    all: try discriminate.
-    inversion p.
-    subst.
-    apply judge_necessity.
-    apply IHe.
-    assumption.
-  - destruct (infer Γ e) eqn:q.
-    all: try discriminate.
-    cbn in *.
-    destruct t.
-    all: try discriminate.
-    cbn in *.
-    destruct (string_dec κ κ0).
-    all: try discriminate.
-    cbn in *.
-    inversion p.
-    subst.
-    apply judge_ext.
-    apply IHe.
-    assumption.
-  - destruct (infer Γ e) eqn:q.
-    all: try discriminate.
-    destruct t.
-    all: try discriminate.
-    inversion p.
-    subst.
-    apply judge_dup.
-    apply IHe.
-    assumption.
-  - destruct (infer Γ e) eqn:q.
-    all: try discriminate.
-    inversion p.
-    subst.
-    apply judge_box.
-    apply IHe.
-    assumption.
-  - destruct (infer Γ e1) eqn:q1.
-    all: try discriminate.
-    cbn in *.
-    destruct t.
-    all: try discriminate.
-    cbn in *.
-    destruct (infer ((x, t) :: Γ) e2) eqn:q2.
-    all: try discriminate.
-    cbn in *.
-    destruct t0.
-    all: try discriminate.
-    cbn in *.
-    destruct (string_dec κ κ0).
-    all: try discriminate.
-    cbn in *.
-    inversion p.
-    subst.
-    eapply judge_bind.
-    Unshelve.
-    3: apply t.
-    + apply IHe1.
-      assumption.
-    + apply IHe2.
-      assumption.
-  - inversion p.
-    subst.
-    apply judge_id.
-  - destruct (infer Γ e1) eqn:q1.
-    all: try discriminate.
-    cbn in *.
-    destruct (infer Γ e2) eqn:q2.
-    all: try discriminate.
-    cbn in *.
-    destruct t.
-    cbn in *.
-    all: try discriminate.
-    cbn in *.
-    destruct t0.
-    all: try discriminate.
-    cbn in *.
-    destruct (string_dec κ μ0).
-    all: try discriminate.
-    cbn in *.
-    inversion p.
-    subst.
-    eapply judge_compose.
-    Unshelve.
-    3: apply μ0.
-    + apply IHe1.
-      assumption.
-    + apply IHe2.
-      assumption.
-  - destruct (infer Γ e) eqn:q.
-    all: try discriminate.
-    cbn in *.
-    destruct t.
-    all: try discriminate.
-    cbn in *.
-    inversion p.
-    subst.
-    apply judge_sym.
-    apply IHe.
-    assumption.
-  - destruct (infer Γ e1) eqn:q1.
-    all: try discriminate.
-    cbn in *.
-    destruct (infer Γ e2) eqn:q2.
-    all: try discriminate.
-    cbn in *.
-    destruct t.
-    all: try discriminate.
-    cbn in *.
-    destruct t0.
-    all: try discriminate.
-    cbn in *.
-    destruct (string_dec κ κ0).
-    all: try discriminate.
-    cbn in *.
-    inversion p.
-    subst.
-    eapply judge_cast_pos.
-    Unshelve.
-    3: apply κ0.
-    + apply IHe1.
-      assumption.
-    + apply IHe2.
-      assumption.
-  - destruct (infer Γ e1) eqn:q1.
-    all: try discriminate.
-    cbn in *.
-    destruct (infer Γ e2) eqn:q2.
-    all: try discriminate.
-    cbn in *.
-    destruct t.
-    all: try discriminate.
-    cbn in *.
-    destruct t0.
-    all: try discriminate.
-    cbn in *.
-    destruct (string_dec κ κ0).
-    all: try discriminate.
-    inversion p.
-    subst.
-    eapply judge_cast_nec.
-    Unshelve.
-    3: apply κ0.
-    + apply IHe1.
-      assumption.
-    + apply IHe2.
-      assumption.
-Defined.
-
-Definition typed (e: tm): if infer [] e is Some τ then ofty τ else True.
-Proof.
-  destruct (infer [] e) eqn:q.
-  - exists e.
-    apply infer_sound.
-    assumption.
-  - apply I.
-Defined.
-
-Example tt_typed: ofty unit := typed tt.
-Example id_typed A: ofty (exp A A) := typed (lam "x" A (var "x")).
-Example compose_typed: ofty _ := typed (id "κ" ∘ id "κ").
-Example id_tt: ofty _ := typed (app (lam "x" unit (var "x")) tt).
-
-Definition includes (Γ Δ: ctx): Prop :=
-  ∀ x τ, maps Δ x τ → maps Γ x τ.
-
-Notation "Γ ⊑ Δ" := (includes Γ Δ) (at level 90).
-
-Instance include_refl: Reflexive includes.
-Proof.
-  intros ? ? ? ?.
-  assumption.
-Qed.
-
-Instance include_trans: Transitive includes.
-Proof.
-  intros ? ? ? p q ? ? ?.
-  unfold includes in *.
-  apply p.
-  apply q.
-  auto.
-Qed.
-
-Theorem weakest {Γ: ctx}: Γ ⊑ [].
-Proof.
-  intros ? ? p.
-  inversion p.
-Qed.
-
-Close Scope string_scope.
-
-(* Lemma weaken {x τ Γ}: (x, τ) :: Γ ⊑ [(x, τ)]. *)
-(* Proof. *)
-(*   intros ? ? p. *)
-(*   induction Γ. *)
-(*   1: assumption. *)
-(*   cbn in *. *)
-(*   inversion p. *)
-(*   all: subst. *)
-(*   - inversion IHΓ. *)
-(*     all: subst. *)
-(*     + constructor. *)
-(*     + constructor. *)
-(*   - inversion p. *)
-(*     all: subst. *)
-(*     all: constructor. *)
-(*     all: auto. *)
-(*     inversion IHΓ. *)
-(*     all: subst. *)
-(*     all: try contradiction. *)
-    
-    
-(*   cbn in *. *)
-(*   destruct (string_dec x x0). *)
-(*   - subst. *)
-(*     reflexivity. *)
-(*   - contradiction. *)
-(* Qed. *)
-
-Theorem weaken_judge {Γ Δ} {e: tm} {τ}:
-    Γ ⊑ Δ →
-    Δ ⊢ e ∈ τ → Γ ⊢ e ∈ τ.
-Proof.
-  intros p ty.
-  generalize dependent Γ.
-  induction ty.
-  all: intros.
-  all: econstructor.
-  all: eauto.
-  - apply IHty.
-    intros ? ? ?.
-    apply lookup_sound.
-    destruct (string_dec x x0) eqn:q.
-    all: subst.
-    + set (p' := lookup_complete H).
-      cbn in *.
-      rewrite q in *.
-      assumption.
-    + set (p' := lookup_complete H).
-      cbn in *.
-      rewrite q in *.
-      apply lookup_complete.
-      apply p.
-      apply lookup_sound.
-      assumption.
-  - apply IHty2.
-    intros ? ? ?.
-    apply lookup_sound.
-    cbn.
-    destruct (string_dec x x0) eqn:q.
-    all: subst.
-    + set (p' := lookup_complete H).
-      cbn in *.
-      rewrite q in p'.
-      assumption.
-    + set (p' := lookup_complete H).
-      cbn in *.
-      rewrite q in p'.
-      apply lookup_complete.
-      apply p.
-      apply lookup_sound.
-      assumption.
-Defined.
-
-Variant whnf: tm → Type :=
-| whnf_set: whnf set
-| whnf_type: whnf type
-
-| whnf_unit: whnf unit
-| whnf_prod A B: whnf (prod A B)
-| whnf_exp A B: whnf (exp A B)
-| whnf_pos κ A: whnf (◇ κ, A)
-| whnf_nec κ A: whnf (□ κ, A)
-| whnf_eq κ μ: whnf (κ ~ μ)
-
-| whnf_tt: whnf tt
-| whnf_fanout e0 e1: whnf (fanout e0 e1)
-| whnf_lam x τ e: whnf (lam x τ e)
-| whnf_box κ e: whnf (box κ e)
-| whnf_necessity κ e: whnf (necessity κ e)
-| whnf_id κ: whnf (id κ)
-.
-
-Variant cd: tm → Type :=
-| cd_app e0 e1: cd (app e0 e1)
-| cd_π1 e: cd (π1 e)
-| cd_π2 e: cd (π2 e)
-| cd_ext κ e: cd (ext κ e)
-| cd_dup e: cd (dup e)
-| cd_bind e0 x e1: cd (bind e0 x e1)
-| cd_compose e0 e1: cd (e0 ∘ e1)
-| cd_sym e: cd (sym e)
-| cd_cast_pos e0 e1: cd (cast_pos e0 e1)
-| cd_cast_nec e0 e1: cd (cast_nec e0 e1)
-.
-
-Lemma canonical {v: tm} {τ}:
-  [] ⊢ v ∈ τ → whnf v →
-  match τ with
-  | unit => (v = tt: Type)
-  | prod _ _ => Σ e0 e1, v = fanout e0 e1
-  | exp τ0 _ => Σ x e0, v = lam x τ0 e0
-  | pos κ _ => Σ e, v = box κ e
-  | nec κ _ => Σ e, v = necessity κ e
-  | eq κ0 κ1 => (κ0 = κ1) ∧ v = id κ0
-  | type => v = set
-  | set => True (* Feels wrong *)
-  | _ => (False: Type)
-  end.
-Proof.
-  intros p w.
-  destruct τ.
-  all: destruct w.
-  all: inversion p.
-  all: subst.
-  all: eauto.
-  - exists e0.
-    exists e1.
-    reflexivity.
-  - exists x.
-    exists e.
-    reflexivity.
-  - exists e.
-    reflexivity.
-  - exists e.
-    reflexivity.
-Defined.
-
 Reserved Notation "'[' x ':=' s ']' t" (at level 20).
 
-Section subst.
-  Context (x: string) (s: tm).
-  Fixpoint subst (ev: tm): tm :=
-    match ev with
-    | var y => if string_dec x y then s else ev
+Function subst x s (ev: tm): tm :=
+  match ev with
+  | var y => if string_dec x y then s else ev
 
-    | lam y τ e => if string_dec x y then ev else lam y τ (subst e)
-    | bind e0 y e1 =>
-      bind (subst e0) y (if string_dec x y then e1 else subst e1)
+  | lam y τ e =>
+    if string_dec x y
+    then
+      lam y (subst x s τ) e
+    else
+      lam y (subst x s τ) (subst x s e)
+  | bind e0 y e1 =>
+    if string_dec x y
+    then
+      bind (subst x s e0) y e1
+    else
+      bind (subst x s e0) y (subst x s e1)
 
-    | tt => ev
+  | tt => ev
 
-    | app e0 e1 => app (subst e0) (subst e1)
+  | app e0 e1 => app (subst x s e0) (subst x s e1)
 
-    | fanout e0 e1 => fanout (subst e0) (subst e1)
-    | π1 e => π1 (subst e)
-    | π2 e => π2 (subst e)
+  | fanout e0 e1 => fanout (subst x s e0) (subst x s e1)
+  | π1 e => π1 (subst x s e)
+  | π2 e => π2 (subst x s e)
 
-    | necessity κ e => necessity κ (subst e)
+  | necessity κ e => necessity κ (subst x s e)
 
-    | ext κ e => ext κ (subst e)
-    | dup e => dup (subst e)
+  | ext κ e => ext κ (subst x s e)
+  | dup e => dup (subst x s e)
 
-    | box κ e => box κ (subst e)
+  | box κ e => box κ (subst x s e)
 
-    | id κ => id κ
-    | e0 ∘ e1 => (subst e0) ∘ (subst e1)
-    | sym e => sym (subst e)
+  | id κ => id κ
+  | e0 ∘ e1 => (subst x s e0) ∘ (subst x s e1)
+  | sym e => sym (subst x s e)
 
-    | cast_pos e0 e1 => cast_pos (subst e0) (subst e1)
-    | cast_nec e0 e1 => cast_nec (subst e0) (subst e1)
+  | cast_pos e0 e1 => cast_pos (subst x s e0) (subst x s e1)
+  | cast_nec e0 e1 => cast_nec (subst x s e0) (subst x s e1)
 
-    | set => set
-    | type => type
+  | set => set
+  | type => type
 
-    | unit => unit
-    | prod e0 e1 => prod (subst e0) (subst e1)
-    | exp e0 e1 => exp (subst e0) (subst e1)
-    | (◇ κ, e) => ◇ κ, (subst e)
-    | (□ κ, e) => □ κ, (subst e)
-    | (κ ~ μ) => κ ~ μ
-    end.
-End subst.
+  | unit => unit
+  | prod e0 e1 => prod (subst x s e0) (subst x s e1)
+  | exp e0 e1 => exp (subst x s e0) (subst x s e1)
+  | (◇ κ, e) => ◇ κ, (subst x s e)
+  | (□ κ, e) => □ κ, (subst x s e)
+  | (κ ~ μ) => κ ~ μ
+  end.
 
 Notation "'[' x ':=' s ']' t" := (subst x s t) .
 
-Theorem subst_type {Γ x} {e0 e1: tm} {τ0 τ1}:
-  (x, τ1) :: Γ ⊢ e0 ∈ τ0 →
-  nil ⊢ e1 ∈ τ1 →
-  Γ ⊢ [x:=e1]e0 ∈ τ0.
-Proof.
-  intros p q.
-  generalize dependent Γ.
-  generalize dependent τ0.
-  induction e0.
-  all: intros.
-  all: inversion p.
-  all: subst.
-  all: try econstructor.
-  all: try eauto.
-  - cbn in *.
-    destruct (string_dec x x0) eqn:r.
-    + cbn in *.
-      set (p' := infer_complete p).
-      cbn in *.
-      subst.
-      rewrite r in p'.
-      cbn in *.
-      subst.
-      inversion p'.
-      subst.
-      refine (weaken_judge _ q).
-      apply weakest.
-    + cbn in *.
-      set (p' := infer_complete p).
-      cbn in *.
-      rewrite r in p'.
-      apply judge_var.
-      apply lookup_sound.
-      assumption.
-  - cbn in *.
-    destruct (string_dec x x0).
-    + subst.
-      apply judge_lam.
-      refine (weaken_judge _ H3).
-      intros ? ? ?.
-      apply lookup_sound.
-      destruct (string_dec x0 x) eqn:t.
-      all: subst.
-      * set (r := lookup_complete H).
-        cbn in *.
-        rewrite t in *.
-        cbn in *.
-        assumption.
-      * set (r := lookup_complete H).
-        cbn in *.
-        rewrite t in *.
-        cbn in *.
-        assumption.
-    + apply judge_lam.
-      apply IHe0_2.
-      refine (weaken_judge _ H3).
-      intros ? ? ?.
-      apply lookup_sound.
-      cbn.
-      destruct (string_dec x x1) eqn:t, (string_dec x0 x1) eqn:u.
-      all: subst.
-      * set (r := lookup_complete H).
-        cbn in *.
-        rewrite t in *.
-        contradiction.
-      * set (r := lookup_complete H).
-        cbn in *.
-        rewrite t in *.
-        rewrite u in *.
-        assumption.
-      * set (r := lookup_complete H).
-        cbn in *.
-        rewrite t in *.
-        rewrite u in *.
-        assumption.
-      * set (r := lookup_complete H).
-        cbn in *.
-        rewrite t in *.
-        rewrite u in *.
-        assumption.
-  - cbn.
-    apply IHe0.
-    refine (weaken_judge _ H2).
-    intros ? ? ?.
-    inversion H.
-  - destruct (string_dec x x0).
-    + subst.
-      refine (weaken_judge _ H4).
-      intros ? ? ?.
-      apply lookup_sound.
-      destruct (string_dec x0 x) eqn:t.
-      all: subst.
-      * set (r := lookup_complete H).
-        cbn in *.
-        rewrite t in *.
-        cbn in *.
-        assumption.
-      * set (r := lookup_complete H).
-        cbn in *.
-        rewrite t in *.
-        cbn in *.
-        assumption.
-    + apply IHe0_2.
-      cbn in *.
-      refine (weaken_judge _ H4).
-      intros ? ? ?.
-      apply lookup_sound.
-      cbn in *.
-      destruct (string_dec x x1) eqn:t.
-      all: subst.
-      * set (r := lookup_complete H).
-        cbn in *.
-        rewrite t in *.
-        cbn in *.
-        destruct (string_dec x0 x1).
-        all: auto.
-        subst.
-        contradiction.
-      * set (r := lookup_complete H).
-        cbn in *.
-        rewrite t in *.
-        cbn in *.
-        assumption.
-Defined.
 
 Reserved Notation "t '~>' t'" (at level 40).
 
@@ -1124,6 +236,545 @@ Inductive step: tm → tm → Type :=
     cast_nec e0 e1 ~> cast_nec e0 e1'
 
 where "A '~>' B" := (step A B).
+
+
+Definition ctx := list (string * tm).
+
+Inductive maps: ctx → string → tm → Prop :=
+| maps_head {Γ x τ}: maps ((x, τ) :: Γ) x τ
+| maps_tail {Γ x y τ τ0}:
+    y ≠ x →
+    maps Γ x τ →
+    maps ((y, τ0) :: Γ) x τ
+.
+
+Reserved Notation "Γ ⊢ e ∈ τ" (at level 80).
+
+Inductive judge (Γ: ctx): tm → tm → Type :=
+| judge_var x τ:
+    maps Γ x τ →
+    Γ ⊢ var x ∈ τ
+
+| judge_set:
+    Γ ⊢ set ∈ type
+| judge_unit:
+    Γ ⊢ unit ∈ set
+| judge_prod A B:
+    Γ ⊢ A ∈ set → Γ ⊢ B ∈ set →
+    Γ ⊢ prod A B ∈ set
+| judge_exp A B:
+    Γ ⊢ A ∈ set → Γ ⊢ B ∈ set →
+    Γ ⊢ exp A B ∈ set
+| judge_pos κ A:
+    Γ ⊢ A ∈ set →
+    Γ ⊢ ◇ κ, A ∈ set
+| judge_nec κ A:
+    Γ ⊢ A ∈ set →
+    Γ ⊢ □ κ, A ∈ set
+| judge_eq κ0 κ1:
+    Γ ⊢ (κ0 ~ κ1) ∈ set
+
+| judge_tt:
+    Γ ⊢ tt ∈ unit
+| judge_fanout e0 e1 τ0 τ1:
+    Γ ⊢ e0 ∈ τ0 → Γ ⊢ e1 ∈ τ1 →
+    Γ ⊢ fanout e0 e1 ∈ (τ0 × τ1)
+
+| judge_π1 e τ0 τ1:
+    Γ ⊢ e ∈ (τ0 × τ1) →
+    Γ ⊢ π1 e ∈ τ0
+| judge_π2 e τ0 τ1:
+    Γ ⊢ e ∈ (τ0 × τ1) →
+    Γ ⊢ π2 e ∈ τ1
+
+| judge_lam e τ0 τ1 x:
+    Γ ⊢ τ0 ∈ set → (x, τ0) :: Γ ⊢ e ∈ τ1 →
+    Γ ⊢ lam x τ0 e ∈ (exp τ0 τ1)
+| judge_app e0 e1 τ0 τ1:
+    Γ ⊢ e0 ∈ (exp τ0 τ1) → Γ ⊢ e1 ∈ τ0 →
+    Γ ⊢ app e0 e1 ∈ τ1
+
+| judge_necessity κ e τ:
+    nil ⊢ e ∈ τ →
+    Γ ⊢ necessity κ e ∈ (□ κ, τ)
+
+| judge_ext κ e τ:
+    Γ ⊢ e ∈ (□ κ, τ) →
+    Γ ⊢ ext κ e ∈ τ
+| judge_dup κ e τ:
+    Γ ⊢ e ∈ (□ κ, τ) →
+    Γ ⊢ dup e ∈ (□ κ, □ κ, τ)
+
+| judge_box κ e τ:
+    Γ ⊢ e ∈ τ →
+    Γ ⊢ box κ e ∈ (◇ κ, τ)
+
+| judge_bind e0 e1 x κ τ0 τ1:
+    Γ ⊢ e0 ∈ (◇ κ, τ0) → (x, τ0) :: Γ ⊢ e1 ∈ (◇ κ, τ1) →
+    Γ ⊢ bind e0 x e1 ∈ (◇ κ, τ1)
+
+| judge_id κ:
+    Γ ⊢ id κ ∈ (κ ~ κ)
+
+| judge_compose e0 e1 κ0 κ1 κ2:
+    Γ ⊢ e0 ∈ (κ1 ~ κ2) → Γ ⊢ e1 ∈ (κ0 ~ κ1) →
+    Γ ⊢ (e0 ∘ e1) ∈ (κ0 ~ κ2)
+
+| judge_sym e κ0 κ1:
+    Γ ⊢ e ∈ (κ1 ~ κ0) →
+    Γ ⊢ sym e ∈ (κ0 ~ κ1)
+
+(* Really unsure of these as faithful to cylindrical logic *)
+| judge_cast_pos e0 e1 κ0 κ1 τ:
+      Γ ⊢ e0 ∈ (κ0 ~ κ1) → Γ ⊢ e1 ∈ (◇ κ0, τ) →
+      Γ ⊢ cast_pos e0 e1 ∈ (◇ κ1, τ)
+| judge_cast_nec e0 e1 κ0 κ1 τ:
+    Γ ⊢ e0 ∈ (κ0 ~ κ1) →
+    Γ ⊢ e1 ∈ (□ κ0, τ) →
+    Γ ⊢ cast_nec e0 e1 ∈ (□ κ1, τ)
+where "Γ ⊢ e ∈ τ" := (judge Γ e τ).
+
+Record ofty (τ: tm) := {
+  term: tm ;
+  proof: nil ⊢ term ∈ τ ;
+}.
+
+Arguments term {τ}.
+Arguments proof {τ}.
+Coercion term: ofty >-> tm.
+
+
+Function lookup (Γ: ctx) (x:string) :=
+  match Γ with
+  | (y, τ) :: Γ' =>
+    if string_dec y x then Some τ else lookup Γ' x
+  | _ => None
+  end.
+
+Theorem lookup_complete {Γ x τ}:
+  maps Γ x τ →
+  lookup Γ x = Some τ.
+Proof.
+  intro p.
+  induction p.
+  - cbn in *.
+    destruct (string_dec x x).
+    2: contradiction.
+    reflexivity.
+  - cbn in *.
+    destruct (string_dec y x).
+    + subst.
+      contradiction.
+    + assumption.
+Qed.
+
+Theorem lookup_sound {Γ x τ}:
+  lookup Γ x = Some τ →
+  maps Γ x τ.
+Proof.
+  intro p.
+  functional induction (lookup Γ x).
+  all: inversion p.
+  all: subst.
+  all: constructor.
+  all: auto.
+Defined.
+
+Function infer (Γ: ctx) (e: tm): option tm :=
+  match e with
+  | type => None
+
+  | set => Some type
+
+  | unit => Some set
+  | prod A B =>
+    if infer Γ A is Some set
+    then
+      if infer Γ B is Some set
+      then
+        Some set
+      else
+        None
+    else
+      None
+  | exp A B =>
+    if infer Γ A is Some set
+    then
+      if infer Γ B is Some set
+      then
+        Some set
+      else
+        None
+    else
+      None
+  | (◇ _, A) =>
+    if infer Γ A is Some set
+    then
+      Some set
+    else
+      None
+  | (□ _, A) =>
+    if infer Γ A is Some set
+    then
+      Some set
+    else
+      None
+  | (_ ~ _) => Some set
+
+  | fanout e0 e1 =>
+    if infer Γ e0 is Some τ0
+    then
+      if infer Γ e1 is Some τ1
+      then
+        Some (τ0 × τ1)
+      else
+        None
+    else
+      None
+  | π1 e =>
+    if infer Γ e is Some (τ0 × τ1)
+    then Some τ0
+    else None
+  | π2 e =>
+    if infer Γ e is Some (τ0 × τ1)
+    then Some τ1
+    else None
+
+  | box κ e =>
+    if infer Γ e is Some τ
+    then
+      Some (◇ κ, τ)
+    else
+      None
+
+  | var x => lookup Γ x
+
+  | lam x τ0 e =>
+    if infer Γ τ0 is Some set
+    then
+      if infer ((x, τ0) :: Γ) e is Some τ1
+      then
+        Some [τ0, τ1]
+      else
+        None
+    else
+      None
+
+  | app e0 e1 =>
+    if infer Γ e0 is Some (exp τ0 τ1)
+    then
+      if infer Γ e1 is Some τ0'
+      then
+        if tm_eq τ0 τ0'
+        then
+          Some τ1
+        else
+          None
+      else
+        None
+    else
+      None
+
+  | tt => Some unit
+
+
+  | necessity κ e =>
+    if infer [] e is Some τ
+    then
+      Some (□ κ, τ)
+    else
+      None
+
+  | ext κ e =>
+    if infer Γ e is Some (□ κ', τ)
+    then
+      if string_dec κ κ'
+      then
+        Some τ
+      else
+        None
+    else
+      None
+  | dup e =>
+    if infer Γ e is Some (□ κ, τ)
+    then
+      Some (□ κ, □ κ, τ)
+    else
+      None
+
+
+  | bind e0 x e1 =>
+    if infer Γ e0 is Some (◇ κ0, τ0)
+    then
+      if infer ((x, τ0) :: Γ) e1 is Some (◇ κ1, τ1)
+      then
+        if string_dec κ0 κ1
+        then
+          Some (◇ κ1, τ1)
+        else
+          None
+      else
+        None
+    else
+      None
+
+  | id κ => Some (κ ~ κ)
+  | e0 ∘ e1 =>
+    if infer Γ e0 is Some (κ1 ~ κ2)
+    then
+      if infer Γ e1 is Some (κ0 ~ κ1')
+      then
+        if string_dec κ1 κ1'
+        then
+          Some (κ0 ~ κ2)
+        else
+          None
+      else
+        None
+    else
+      None
+
+  | sym e =>
+    if infer Γ e is Some (κ0 ~ κ1)
+    then
+      Some (κ1 ~ κ0)
+    else
+      None
+
+  | cast_pos e0 e1 =>
+    if infer Γ e0 is Some (κ0 ~ κ1)
+    then
+      if infer Γ e1 is Some (◇ κ0', τ)
+      then
+        if string_dec κ0 κ0'
+        then
+          Some (◇ κ1, τ)
+        else
+          None
+      else
+        None
+    else
+      None
+
+  | cast_nec e0 e1 =>
+    if infer Γ e0 is Some (κ0 ~ κ1)
+    then
+      if infer Γ e1 is Some (□ κ0', τ)
+      then
+        if string_dec κ0 κ0'
+        then
+          Some (□ κ1, τ)
+        else
+          None
+      else
+        None
+    else
+      None
+  end.
+
+Theorem infer_complete {Γ e τ}:
+  Γ ⊢ e ∈ τ → infer Γ e = Some τ.
+  intro p.
+  induction p.
+  all: cbn in *.
+  all: auto.
+  all: try rewrite IHp.
+  all: cbn in *.
+  all: try rewrite IHp1.
+  all: cbn in *.
+  all: try rewrite IHp2.
+  all: cbn in *.
+  all: try reflexivity.
+  all: cbn in *.
+  - apply lookup_complete.
+    assumption.
+  - destruct (tm_eq τ0 τ0).
+    2: contradiction.
+    reflexivity.
+  - destruct (string_dec κ κ).
+    2: contradiction.
+    reflexivity.
+  - destruct (string_dec κ κ).
+    2: contradiction.
+    reflexivity.
+  - destruct (string_dec κ1 κ1).
+    2: contradiction.
+    reflexivity.
+  - destruct (string_dec κ0 κ0).
+    2: contradiction.
+    reflexivity.
+  - destruct (string_dec κ0 κ0).
+    2: contradiction.
+    reflexivity.
+Qed.
+
+Theorem infer_sound {Γ e τ}:
+  infer Γ e = Some τ → Γ ⊢ e ∈ τ.
+Proof.
+  generalize dependent τ.
+  functional induction (infer Γ e).
+  all: intros τ'.
+  all: intros p.
+  all: try discriminate.
+  all: inversion p.
+  all: subst.
+  all: econstructor.
+  all: eauto.
+  apply lookup_sound.
+  auto.
+Defined.
+
+Definition typed (e: tm): if infer [] e is Some τ then ofty τ else True.
+Proof.
+  destruct (infer [] e) eqn:q.
+  - exists e.
+    apply infer_sound.
+    assumption.
+  - apply I.
+Defined.
+
+Example tt_typed: ofty unit := typed tt.
+Example id_typed: ofty (exp unit unit) := typed (lam "x" unit (var "x")).
+Example compose_typed: ofty _ := typed (id "κ" ∘ id "κ").
+Example id_tt: ofty _ := typed (app (lam "x" unit (var "x")) tt).
+
+Definition includes (Γ Δ: ctx): Prop :=
+  ∀ x τ, maps Δ x τ → maps Γ x τ.
+
+Notation "Γ ⊑ Δ" := (includes Γ Δ) (at level 90).
+
+Instance include_refl: Reflexive includes.
+Proof.
+  intros ? ? ? ?.
+  assumption.
+Qed.
+
+Instance include_trans: Transitive includes.
+Proof.
+  intros ? ? ? p q ? ? ?.
+  unfold includes in *.
+  apply p.
+  apply q.
+  auto.
+Qed.
+
+Theorem weakest {Γ: ctx}: Γ ⊑ nil.
+Proof.
+  intros ? ? p.
+  inversion p.
+Qed.
+
+Close Scope string_scope.
+
+Theorem weaken_judge {Γ Δ} {e: tm} {τ}:
+    Γ ⊑ Δ →
+    Δ ⊢ e ∈ τ → Γ ⊢ e ∈ τ.
+Proof.
+  intros p ty.
+  generalize dependent Γ.
+  induction ty.
+  all: intros.
+  all: econstructor.
+  all: eauto.
+  - apply IHty2.
+    intros ? ? ?.
+    apply lookup_sound.
+    destruct (string_dec x x0) eqn:q.
+    all: subst.
+    + set (p' := lookup_complete H).
+      cbn in *.
+      rewrite q in *.
+      assumption.
+    + set (p' := lookup_complete H).
+      cbn in *.
+      rewrite q in *.
+      apply lookup_complete.
+      apply p.
+      apply lookup_sound.
+      assumption.
+  - apply IHty2.
+    intros ? ? ?.
+    apply lookup_sound.
+    cbn.
+    destruct (string_dec x x0) eqn:q.
+    all: subst.
+    + set (p' := lookup_complete H).
+      cbn in *.
+      rewrite q in p'.
+      assumption.
+    + set (p' := lookup_complete H).
+      cbn in *.
+      rewrite q in p'.
+      apply lookup_complete.
+      apply p.
+      apply lookup_sound.
+      assumption.
+Defined.
+
+Variant whnf: tm → Type :=
+| whnf_set: whnf set
+| whnf_type: whnf type
+
+| whnf_unit: whnf unit
+| whnf_prod A B: whnf (prod A B)
+| whnf_exp A B: whnf (exp A B)
+| whnf_pos κ A: whnf (◇ κ, A)
+| whnf_nec κ A: whnf (□ κ, A)
+| whnf_eq κ μ: whnf (κ ~ μ)
+
+| whnf_tt: whnf tt
+| whnf_fanout e0 e1: whnf (fanout e0 e1)
+| whnf_lam x τ e: whnf (lam x τ e)
+| whnf_box κ e: whnf (box κ e)
+| whnf_necessity κ e: whnf (necessity κ e)
+| whnf_id κ: whnf (id κ)
+.
+
+Variant cd: tm → Type :=
+| cd_app e0 e1: cd (app e0 e1)
+| cd_π1 e: cd (π1 e)
+| cd_π2 e: cd (π2 e)
+| cd_ext κ e: cd (ext κ e)
+| cd_dup e: cd (dup e)
+| cd_bind e0 x e1: cd (bind e0 x e1)
+| cd_compose e0 e1: cd (e0 ∘ e1)
+| cd_sym e: cd (sym e)
+| cd_cast_pos e0 e1: cd (cast_pos e0 e1)
+| cd_cast_nec e0 e1: cd (cast_nec e0 e1)
+.
+
+Lemma canonical {v: tm} {τ}:
+  nil ⊢ v ∈ τ → whnf v →
+  match τ with
+  | unit => (v = tt: Type)
+  | prod _ _ => Σ e0 e1, v = fanout e0 e1
+  | exp τ0 _ => Σ x e0, v = lam x τ0 e0
+  | pos κ _ => Σ e, v = box κ e
+  | nec κ _ => Σ e, v = necessity κ e
+  | eq κ0 κ1 => (κ0 = κ1) ∧ v = id κ0
+  | type => v = set
+  | set => True (* Feels wrong *)
+  | _ => (False: Type)
+  end.
+Proof.
+  intros p w.
+  destruct τ.
+  all: destruct w.
+  all: inversion p.
+  all: subst.
+  all: eauto.
+  - exists e0.
+    exists e1.
+    reflexivity.
+  - exists x.
+    exists e.
+    reflexivity.
+  - exists e.
+    reflexivity.
+  - exists e.
+    reflexivity.
+Defined.
+
 
 Lemma to_cd {e e': tm}: e ~> e' → cd e.
 Proof.
@@ -1371,6 +1022,133 @@ Proof.
     exists (cast_nec e' e1).
     constructor.
     auto.
+Defined.
+
+Theorem subst_type {Γ x} {e0 e1: tm} {τ0 τ1}:
+  (x, τ1) :: Γ ⊢ e0 ∈ τ0 →
+  nil ⊢ e1 ∈ τ1 →
+  Γ ⊢ [x:=e1]e0 ∈ τ0.
+Proof.
+  intros p q.
+  generalize dependent Γ.
+  generalize dependent τ0.
+  induction e0.
+  all: intros.
+  all: inversion p.
+  all: subst.
+  all: try econstructor.
+  all: try eauto.
+  - cbn in *.
+    destruct (string_dec x x0) eqn:r.
+    + cbn in *.
+      set (p' := infer_complete p).
+      cbn in *.
+      subst.
+      rewrite r in p'.
+      cbn in *.
+      subst.
+      inversion p'.
+      subst.
+      refine (weaken_judge _ q).
+      apply weakest.
+    + cbn in *.
+      set (p' := infer_complete p).
+      cbn in *.
+      rewrite r in p'.
+      apply judge_var.
+      apply lookup_sound.
+      assumption.
+  - cbn in *.
+    destruct (string_dec x x0).
+    + subst.
+      apply judge_lam.
+      refine (weaken_judge _ H3).
+      intros ? ? ?.
+      apply lookup_sound.
+      destruct (string_dec x0 x) eqn:t.
+      all: subst.
+      * set (r := lookup_complete H).
+        cbn in *.
+        rewrite t in *.
+        cbn in *.
+        inversion r.
+        subst.
+        admit.
+      * set (r := lookup_complete H).
+        cbn in *.
+        rewrite t in *.
+        cbn in *.
+        assumption.
+    + apply judge_lam.
+      apply IHe0_2.
+      refine (weaken_judge _ H3).
+      intros ? ? ?.
+      apply lookup_sound.
+      cbn.
+      destruct (string_dec x x1) eqn:t, (string_dec x0 x1) eqn:u.
+      all: subst.
+      * set (r := lookup_complete H).
+        cbn in *.
+        rewrite t in *.
+        contradiction.
+      * set (r := lookup_complete H).
+        cbn in *.
+        rewrite t in *.
+        rewrite u in *.
+        assumption.
+      * set (r := lookup_complete H).
+        cbn in *.
+        rewrite t in *.
+        rewrite u in *.
+        assumption.
+      * set (r := lookup_complete H).
+        cbn in *.
+        rewrite t in *.
+        rewrite u in *.
+        assumption.
+  - cbn.
+    apply IHe0.
+    refine (weaken_judge _ H2).
+    intros ? ? ?.
+    inversion H.
+  - destruct (string_dec x x0).
+    + subst.
+      refine (weaken_judge _ H4).
+      intros ? ? ?.
+      apply lookup_sound.
+      destruct (string_dec x0 x) eqn:t.
+      all: subst.
+      * set (r := lookup_complete H).
+        cbn in *.
+        rewrite t in *.
+        cbn in *.
+        assumption.
+      * set (r := lookup_complete H).
+        cbn in *.
+        rewrite t in *.
+        cbn in *.
+        assumption.
+    + apply IHe0_2.
+      cbn in *.
+      refine (weaken_judge _ H4).
+      intros ? ? ?.
+      apply lookup_sound.
+      cbn in *.
+      destruct (string_dec x x1) eqn:t.
+      all: subst.
+      * set (r := lookup_complete H).
+        cbn in *.
+        rewrite t in *.
+        cbn in *.
+        destruct (string_dec x0 x1).
+        all: auto.
+        subst.
+        contradiction.
+      * set (r := lookup_complete H).
+        cbn in *.
+        rewrite t in *.
+        cbn in *.
+        assumption.
 Defined.
 
 Theorem preservation (e e': tm) τ:
