coc.v
@@ -1,0 +1,401 @@
+Require Import Coq.Unicode.Utf8.
+Require Import Coq.Lists.List.
+Require Import Coq.Strings.String.
+Require Import Coq.Bool.Bool.
+Require Import Coq.Setoids.Setoid.
+Require Import Coq.Classes.SetoidClass.
+Require Import FunInd.
+Require Import Recdef.
+
+Import IfNotations.
+Import ListNotations.
+Open Scope string_scope.
+
+Close Scope nat.
+
+Reserved Notation "⟨ x , y , .. , z ⟩".
+
+Definition option_bind {A B} (x: option A) (f: A → option B): option B :=
+  if x is Some x' then f x' else None.
+Infix ">>=" := option_bind (at level 30, right associativity).
+
+Definition option_then {A B} (x: option A) (y: option B): option B :=
+  if x is Some _ then y else None.
+
+Infix ">>" := option_then (at level 30, right associativity).
+
+Reserved Notation "f ∘ g" (at level 30).
+
+Inductive tm: Type :=
+| var (x: string)
+
+| set
+| type
+
+| all (x: string) (s: tm) (e: tm)
+| lam (x: string) (s: tm) (e: tm)
+| app (f x: tm)
+.
+
+Arguments tm: clear implicits.
+
+Definition tm_eq (x y: tm): {x = y} + {x ≠ y}.
+Proof.
+  set (s := string_dec).
+  decide equality.
+Defined.
+
+
+Reserved Notation "'[' x ':=' s ']' t" (at level 20).
+
+Function subst (x: string) (s: tm) (ev: tm): tm :=
+  match ev with
+  | var y =>
+    if string_dec x y then s else ev
+
+  | all y τ e =>
+    if string_dec x y
+    then
+      ev
+    else
+      all y (subst x s τ) (subst x s e)
+  | lam y τ e =>
+    if string_dec x y
+    then
+      lam y (subst x s τ) e
+    else
+      lam y (subst x s τ) (subst x s e)
+
+  | app e0 e1 => app (subst x s e0) (subst x s e1)
+
+  | set => set
+  | type => type
+  end.
+
+Notation "'[' x ':=' s ']' t" := (subst x s t) .
+
+
+Definition ctx := list (string * tm).
+
+Inductive maps: ctx → string → tm → Prop :=
+| maps_head {Γ x τ}: maps ((x, τ) :: Γ) x τ
+| maps_tail {Γ x y τ τ0}:
+    y ≠ x →
+    maps Γ x τ →
+    maps ((y, τ0) :: Γ) x τ
+.
+
+Reserved Notation "Γ ⊢ e0 ▹ e1" (at level 80).
+Reserved Notation "Γ ⊢ e ∈ τ" (at level 80).
+
+(* FIXME *)
+Inductive convertable (Γ: ctx): relation tm :=
+| reflexive: reflexive tm (convertable Γ)
+| transitive: transitive tm (convertable Γ)
+
+(* FIXME enforce fresh vars ? *)
+(* FIXME enforce maps ? *)
+| alpha_conversion {x y e}: Γ ⊢ e ▹ [x := y] e
+
+| beta_reduction {x t T u}: Γ ⊢ app (lam x T t) u ▹ [x := u] t
+| eta_expansion {x t T}:
+    Γ ⊢ t ▹ all x T (app t (var x))
+where "Γ ⊢ e0 ▹ e1" := (convertable Γ e0 e1).
+
+Instance convertable_PreOrder Γ: PreOrder (convertable Γ).
+Proof.
+  exists.
+  - intros ?.
+    apply reflexive.
+  - intros ? ? ? p q.
+    apply (transitive _ _ _ _ p).
+    assumption.
+Qed.
+
+Definition definitionally_equal (Γ: ctx): relation tm :=
+  λ e0 e1,
+  ∃ u,
+    (* FIXME, Not quite right *)
+    Γ ⊢ e0 ▹ u ∧ Γ ⊢ e1 ▹ u.
+
+Notation "Γ ⊢ e0 = e1" := (definitionally_equal Γ e0 e1) (at level 80).
+
+Inductive judge (Γ: ctx): tm → tm → Type :=
+| judge_var {x τ}:
+    maps Γ x τ →
+    Γ ⊢ var x ∈ τ
+
+| judge_set:
+    Γ ⊢ set ∈ type
+
+| judge_all {x A B K L}:
+    Γ ⊢ A ∈ K → (x, A) :: Γ ⊢ B ∈ L →
+    Γ ⊢ all x A B ∈ L
+| judge_lam {x A B K N}:
+    Γ ⊢ A ∈ K → (x, A) :: Γ ⊢ N ∈ B →
+    Γ ⊢ lam x A N ∈ (all x A B)
+| judge_app {M N A B x}:
+    Γ ⊢ M ∈ (all x A B) → Γ ⊢ N ∈ A →
+    Γ ⊢ app M N ∈ [x:=N]B
+
+(* | judge_convert {M A B K}: *)
+(*     Γ ⊢ M ∈ A → Γ ⊢ A ▹ B → Γ ⊢ B ∈ K → *)
+(*     Γ ⊢ M ∈ B *)
+where "Γ ⊢ e ∈ τ" := (judge Γ e τ).
+
+Reserved Notation "t '~>' t'" (at level 40).
+
+Record ofty (τ: tm) := {
+  term: tm ;
+  proof: nil ⊢ term ∈ τ ;
+}.
+
+Arguments term {τ}.
+Arguments proof {τ}.
+Coercion term: ofty >-> tm.
+
+Function lookup (Γ: ctx) (x:string) :=
+  match Γ with
+  | (y, τ) :: Γ' =>
+    if string_dec y x then Some τ else lookup Γ' x
+  | _ => None
+  end.
+
+Theorem lookup_complete {Γ x τ}:
+  maps Γ x τ →
+  lookup Γ x = Some τ.
+Proof.
+  intro p.
+  induction p.
+  - cbn in *.
+    destruct (string_dec x x).
+    2: contradiction.
+    reflexivity.
+  - cbn in *.
+    destruct (string_dec y x).
+    + subst.
+      contradiction.
+    + assumption.
+Qed.
+
+Theorem lookup_sound {Γ x τ}:
+  lookup Γ x = Some τ →
+  maps Γ x τ.
+Proof.
+  intro p.
+  functional induction (lookup Γ x).
+  all: inversion p.
+  all: subst.
+  all: constructor.
+  all: auto.
+Defined.
+
+Function infer (Γ: ctx) (e: tm): option tm :=
+  match e with
+  | type => None
+
+  | set => Some type
+
+  | var x => lookup Γ x
+
+  | all x A B =>
+    if infer Γ A is Some K
+    then
+      if infer ((x, A) :: Γ) B is Some L
+      then
+        Some L
+      else
+        None
+    else
+      None
+
+  | lam x A N =>
+    if infer Γ A is Some K
+    then
+      if infer ((x, A) :: Γ) N is Some B
+      then
+        Some (all x A B)
+      else
+        None
+    else
+      None
+
+  | app M N =>
+    if infer Γ M is Some (all x A B)
+    then
+      if infer Γ N is Some A'
+      then
+        if tm_eq A A'
+        then
+          Some ([x := N] B)
+        else
+          None
+      else
+        None
+    else
+      None
+  end.
+
+Theorem infer_complete {Γ e τ}:
+  Γ ⊢ e ∈ τ →
+  infer Γ e = Some τ.
+  intro p.
+  induction p.
+  - cbn.
+    rewrite (lookup_complete m).
+    reflexivity.
+  - cbn.
+    reflexivity.
+  - cbn in *.
+    rewrite IHp1, IHp2.
+    cbn.
+    reflexivity.
+  - cbn in *.
+    rewrite IHp1, IHp2.
+    cbn.
+    reflexivity.
+  - cbn in *.
+    rewrite IHp1, IHp2.
+    cbn.
+    destruct (tm_eq A A).
+    2: contradiction.
+    cbn.
+    reflexivity.
+Qed.
+
+Theorem infer_sound {Γ e τ}:
+  infer Γ e = Some τ → Γ ⊢ e ∈ τ.
+Proof.
+  generalize dependent τ.
+  functional induction (infer Γ e).
+  all: intros τ.
+  all: intros p.
+  all: try discriminate.
+  all: inversion p.
+  all: subst.
+  all: econstructor.
+  all: eauto.
+  apply lookup_sound.
+  auto.
+Defined.
+
+Definition typed (e: tm): if infer [] e is Some τ then ofty τ else True.
+Proof.
+  destruct (infer [] e) eqn:q.
+  - exists e.
+    apply infer_sound.
+    assumption.
+  - apply I.
+Defined.
+
+Example tt_typed: ofty _ := typed (all "x" set (var "x")).
+Example id_typed: ofty _ := typed (lam "A" set (lam "x" (var "A") (var "x"))).
+
+
+Function eval (e: tm): option tm :=
+  match e with
+  | app (lam x _ e0) e1 => Some ([x := e1] e0)
+
+  | app e0 e1 =>
+    eval e0 >>= λ e0',
+    Some (app e0' e1)
+
+  | _ => None
+  end.
+
+
+Definition includes (Γ Δ: ctx): Prop :=
+  ∀ x τ, maps Δ x τ → maps Γ x τ.
+
+Notation "Γ ⊑ Δ" := (includes Γ Δ) (at level 90).
+
+Instance include_refl: Reflexive includes.
+Proof.
+  intros ? ? ? ?.
+  assumption.
+Qed.
+
+Instance include_trans: Transitive includes.
+Proof.
+  intros ? ? ? p q ? ? ?.
+  unfold includes in *.
+  apply p.
+  apply q.
+  auto.
+Qed.
+
+Theorem weakest {Γ: ctx}: Γ ⊑ nil.
+Proof.
+  intros ? ? p.
+  inversion p.
+Qed.
+
+Close Scope string_scope.
+
+Theorem weaken_judge {Γ Δ} {e: tm} {τ}:
+    Γ ⊑ Δ →
+    Δ ⊢ e ∈ τ → Γ ⊢ e ∈ τ.
+Proof.
+  intros p ty.
+  generalize dependent Γ.
+  induction ty.
+  all: intros.
+  all: econstructor.
+  all: eauto.
+  - apply IHty2.
+    intros ? ? ?.
+    apply lookup_sound.
+    destruct (string_dec x x0) eqn:q.
+    all: subst.
+    + set (p' := lookup_complete H).
+      cbn in *.
+      rewrite q in *.
+      assumption.
+    + set (p' := lookup_complete H).
+      cbn in *.
+      rewrite q in *.
+      apply lookup_complete.
+      apply p.
+      apply lookup_sound.
+      assumption.
+  - apply IHty2.
+    intros ? ? ?.
+    apply lookup_sound.
+    cbn.
+    destruct (string_dec x x0) eqn:q.
+    all: subst.
+    + set (p' := lookup_complete H).
+      cbn in *.
+      rewrite q in p'.
+      assumption.
+    + set (p' := lookup_complete H).
+      cbn in *.
+      rewrite q in p'.
+      apply lookup_complete.
+      apply p.
+      apply lookup_sound.
+      assumption.
+Defined.
+
+Variant whnf: tm → Type :=
+| whnf_set: whnf set
+| whnf_type: whnf type
+
+| whnf_all x A B: whnf (all x A B)
+| whnf_lam x τ e: whnf (lam x τ e)
+.
+
+Variant cd: tm → Type :=
+| cd_app e0 e1: cd (app e0 e1)
+.
+
+
+
+Inductive step: tm → tm → Type :=
+| step_app_lam x τ e0 e1:
+    app (lam x τ e0) e1 ~> [x:=e1]e0
+
+| step_app e0 e1 e0':
+    e0 ~> e0' →
+    app e0 e1 ~> app e0' e1
+where "A '~>' B" := (step A B).
