tarski.v
@@ -1,0 +1,341 @@
+Require Import Coq.Unicode.Utf8.
+Require Import Coq.Lists.List.
+Require Import Coq.Strings.String.
+Require Import Coq.Bool.Bool.
+Require Import Coq.Setoids.Setoid.
+Require Import Coq.Classes.SetoidClass.
+Require Import FunInd.
+Require Import Recdef.
+
+Import IfNotations.
+Import ListNotations.
+Open Scope string_scope.
+
+Close Scope nat.
+
+Reserved Notation "⟨ x , y , .. , z ⟩".
+
+Definition option_bind {A B} (x: option A) (f: A → option B): option B :=
+  if x is Some x' then f x' else None.
+Infix ">>=" := option_bind (at level 30, right associativity).
+
+Definition option_then {A B} (x: option A) (y: option B): option B :=
+  if x is Some _ then y else None.
+
+Infix ">>" := option_then (at level 30, right associativity).
+
+Inductive tm: Type :=
+| set
+| type
+
+| prod (A B: tm)
+| pos (κ: string) (A: tm)
+| eq (κ μ: string)
+
+| fanout (e0 e1: tm)
+| π1 (e: tm)
+| π2 (e: tm)
+
+| box (κ: string) (e: tm)
+| join (κ: string) (e: tm)
+
+| id (κ: string)
+| J (e0 e1: tm)
+.
+
+Arguments tm: clear implicits.
+
+Definition tm_eq (x y: tm): {x = y} + {x ≠ y}.
+Proof.
+  set (s := string_dec).
+  decide equality.
+Defined.
+
+Infix "×" := prod (at level 50).
+
+Notation "'◇' κ , A" := (pos κ A) (at level 200).
+(* (* Like forall but I use box because ∀ is already taken *) *)
+(* Notation "□ κ , A" := (nec κ A) (at level 200). *)
+Infix "~" := eq (at level 90).
+
+Notation "⟨ x , y , .. , z ⟩" := (fanout .. (fanout x y) .. z).
+
+Reserved Notation "'[' x ':=' s ']' t" (at level 20).
+
+Function subst (x: string) (s: string) (ev: tm): tm :=
+  match ev with
+  | fanout e0 e1 => fanout (subst x s e0) (subst x s e1)
+  | π1 e => π1 (subst x s e)
+  | π2 e => π2 (subst x s e)
+
+  | box κ e =>
+    box (if string_dec x κ then s else κ) (subst x s e)
+  | join κ e =>
+    join (if string_dec x κ then s else κ) (subst x s e)
+
+  | id κ => id (if string_dec x κ then s else κ)
+  | J e0 e1 => J (subst x s e0) (subst x s e1)
+
+  | prod e0 e1 => prod (subst x s e0) (subst x s e1)
+
+  | (◇ κ, e) =>
+    ◇ (if string_dec x κ then s else κ), subst x s e
+  | (κ ~ μ) =>
+    (if string_dec x κ then s else κ) ~ (if string_dec x μ then s else x)
+
+  | set => set
+  | type => type
+  end.
+
+
+Notation "'[' x ':=' s ']' t" := (subst x s t) .
+
+Reserved Notation "e ∈ τ" (at level 80).
+
+Inductive tm_equiv: relation tm :=
+| reflexive: reflexive tm tm_equiv
+| symmetric: symmetric tm tm_equiv
+| transitive: transitive tm tm_equiv
+
+| π1_fanout A B: tm_equiv (π1 (fanout A B)) A
+| π2_fanout A B: tm_equiv (π2 (fanout A B)) B
+.
+
+Instance tm_Equivalence: Equivalence tm_equiv.
+Proof.
+  exists.
+  - intros ?.
+    apply reflexive.
+  - intros ? ? ?.
+    apply symmetric.
+    assumption.
+  - intros ? ? ? p q.
+    apply (transitive _ _ _ p).
+    assumption.
+Qed.
+
+Instance tm_Setoid: Setoid tm := {
+  equiv := tm_equiv ;
+}.
+
+Inductive judge: tm → tm → Type :=
+| judge_set:
+    set ∈ type
+
+| judge_prod {A B}:
+    A ∈ set → B ∈ set →
+    prod A B ∈ set
+| judge_eq {κ μ}:
+    (κ ~ μ) ∈ set
+| judge_pos {κ A}:
+    A ∈ set →
+    (◇ κ, A) ∈ set
+
+| judge_fanout {e0 e1 A B}:
+    e0 ∈ A → e1 ∈ B →
+    fanout e0 e1 ∈ (A × B)
+| judge_π1 {e A B}:
+    e ∈ A × B →
+    π1 e ∈ A
+| judge_π2 {e A B}:
+    e ∈ A × B →
+    π2 e ∈ B
+
+| judge_box {κ e A}:
+    e ∈ A →
+    box κ e ∈ ◇ κ, A
+| judge_join {κ e A}:
+    e ∈ (◇ κ, (◇ κ, A)) →
+    join κ e ∈ ◇ κ, A
+
+| judge_id {κ}:
+    id κ ∈ (κ ~ κ)
+
+(* really unsure here *)
+| judge_J {κ0 κ1 e0 e1 τ}:
+    e0 ∈ (κ0 ~ κ1) →
+    e1 ∈ (◇ κ0, τ) →
+    J e0 e1 ∈ (◇ κ1, [κ0 := κ1]τ)
+
+(* | judge_convert {M A B K}: *)
+(*     M ∈ A → A == B → B ∈ K → *)
+(*     M ∈ B *)
+where "e ∈ τ" := (judge e τ).
+
+Record ofty (τ: tm) := {
+  term: tm ;
+  proof: term ∈ τ ;
+}.
+
+Arguments term {τ}.
+Arguments proof {τ}.
+Coercion term: ofty >-> tm.
+
+Function step (ev: tm): tm :=
+  match ev with
+  | π1 (fanout A _) => step A
+  | π2 (fanout _ B) => step B
+
+  | join _ (box _ (box κ e)) => box κ (step e)
+
+  | J (id κ0) (box κ1 e1) => [κ1 := κ0] (step e1)
+
+  | prod A B => prod (step A) (step B)
+  | (◇ κ, A) => ◇ κ, step A
+  | ⟨ e0 , e1 ⟩ => ⟨ step e0 , step e1 ⟩
+  | π1 e => π1 (step e)
+  | π2 e => π2 (step e)
+  | box κ e => box κ (step e)
+  | join κ e => join κ (step e)
+  | J e0 e1 => J (step e0) (step e1)
+
+  | _ => ev
+  end.
+
+Function infer (e: tm): option tm :=
+  match e with
+  | type => None
+
+  | set => Some type
+
+  | prod A B =>
+    if infer A is Some set
+    then
+      if infer B is Some set
+      then
+        Some set
+      else
+        None
+    else
+      None
+  | (◇ _, A) =>
+    if infer A is Some set
+    then
+      Some set
+    else
+      None
+  | (_ ~ _) => Some set
+
+  | ⟨ e0 , e1 ⟩ =>
+    if infer e0 is Some τ0
+    then
+      if infer e1 is Some τ1
+      then
+        Some (τ0 × τ1)
+      else
+        None
+    else
+      None
+  | π1 e =>
+    if infer e is Some (τ0 × τ1)
+    then Some τ0
+    else None
+  | π2 e =>
+    if infer e is Some (τ0 × τ1)
+    then Some τ1
+    else None
+
+  | box κ e =>
+    if infer e is Some τ
+    then
+      Some (◇ κ, τ)
+    else
+      None
+  | join κ e =>
+    if infer e is Some (◇ κ0, ◇ κ1, A)
+    then
+      if string_dec κ κ0
+      then
+        if string_dec κ κ1
+        then
+          Some (◇ κ, A)
+        else
+          None
+      else
+        None
+    else
+      None
+
+  | id κ => Some (κ ~ κ)
+  | J e0 e1 =>
+    if infer e0 is Some (κ0 ~ κ1)
+    then
+      if infer e1 is Some (◇ κ0', τ)
+      then
+        if string_dec κ0 κ0'
+        then
+          Some (◇ κ1, [κ0 := κ1] τ)
+        else
+          None
+      else
+        None
+    else
+      None
+  end.
+
+Theorem infer_complete {e τ}:
+  e ∈ τ →
+  infer e = Some τ.
+  intro p.
+  induction p.
+  all: cbn.
+  all: try reflexivity.
+  - rewrite IHp1, IHp2.
+    cbn.
+    reflexivity.
+  - cbn.
+    rewrite IHp.
+    reflexivity.
+  - cbn.
+    rewrite IHp1, IHp2.
+    cbn.
+    reflexivity.
+  - cbn.
+    rewrite IHp.
+    reflexivity.
+  - cbn.
+    rewrite IHp.
+    reflexivity.
+  - cbn.
+    rewrite IHp.
+    reflexivity.
+  - cbn.
+    rewrite IHp.
+    destruct (string_dec κ κ).
+    2:contradiction.
+    reflexivity.
+  - cbn.
+    rewrite IHp1, IHp2.
+    cbn.
+    destruct (string_dec κ0 κ0).
+    2: contradiction.
+    cbn.
+    reflexivity.
+Qed.
+
+Theorem infer_sound {e τ}:
+  infer e = Some τ → e ∈ τ.
+Proof.
+  generalize dependent τ.
+  functional induction (infer e).
+  all: intros τ'.
+  all: intros p.
+  all: try discriminate.
+  all: inversion p.
+  all: subst.
+  all: econstructor.
+  all: eauto.
+Defined.
+
+Definition typed (e: tm): if infer e is Some τ then ofty τ else True.
+Proof.
+  destruct (infer e) eqn:q.
+  - exists e.
+    apply infer_sound.
+    assumption.
+  - apply I.
+Defined.
+
+Example tt_typed: ofty _ :=
+  typed
+    (J (id "x") (box "x" (◇ "x", "x" ~ "x"))).
